lib/evaluate.ml
@@ -1,304 +1,305 @@
 open Lambda
 
-module Evaluator = struct
-  type lbl = int
+let rec pp exp =
+    match exp with
+    | EVar s
+    | MVar s -> print_string s
+    | Lam (s, e) ->
+        print_string "\\";
+        print_string (s ^ ".");
+        pp e;
+        print_string ""
+    | App (e1, e2) ->
+        print_string "(";
+        pp e1;
+        print_string ") (";
+        pp e2;
+        print_string ")"
+    | Link (e1, e2) ->
+        print_string "(";
+        pp e1;
+        print_string ")!(";
+        pp e2;
+        print_string ")"
+    | Empty -> print_string "ε"
+    | Lete (x, e1, e2)
+    | Letm (x, e1, e2) ->
+      print_string "let ";
+      print_string x;
+      print_string " = ";
+      pp e1;
+      print_string " in ";
+      pp e2
 
-  let num_of_lbls = ref 0
-
-  type loc = int
-
-  let num_of_strings = ref 0
-
-  module LEnv = Map.Make (struct
-    type t = loc
-
-    let compare = compare
-  end)
-
-  type lblexp = LVar of loc | LLam of loc * lbl | LApp of lbl * lbl
-
-  let label_table : (lbl, lblexp) Hashtbl.t = Hashtbl.create 10
-  let string_table : (string, loc) Hashtbl.t = Hashtbl.create 10
-  let location_table : (loc, string) Hashtbl.t = Hashtbl.create 10
-  let de_bruijn : (lbl, int) Hashtbl.t = Hashtbl.create 10
-
-  let new_lbl () =
-    incr num_of_lbls;
-    !num_of_lbls
-
-  let get_loc s =
-    match Hashtbl.find string_table s with
-    | l -> l
-    | exception Not_found ->
-        incr num_of_strings;
-        Hashtbl.add string_table s !num_of_strings;
-        Hashtbl.add location_table !num_of_strings s;
-        !num_of_strings
-
-  let get_string l = Hashtbl.find location_table l
-
-  let rec label (e : lexp) (local_de_bruijn : int LEnv.t) =
-    let lbl = new_lbl () in
-    let lblexp =
-      match e with
-      | Var x ->
-          let x = get_loc x in
-          let idx = try LEnv.find x local_de_bruijn with _ -> -1 in
-          Hashtbl.add de_bruijn lbl idx;
-          LVar x
-      | Lam (x, e) ->
-          let x = get_loc x in
-          let updated_de_bruijn =
-            LEnv.map (fun index -> index + 1) local_de_bruijn
-          in
-          let lbl = label e (LEnv.add x 0 updated_de_bruijn) in
-          LLam (x, lbl)
-      | App (e1, e2) ->
-          let lbl1 = label e1 local_de_bruijn in
-          let lbl2 = label e2 local_de_bruijn in
-          LApp (lbl1, lbl2)
-    in
-    Hashtbl.add label_table lbl lblexp;
-    lbl
-
-  type t = A of t LEnv.t * lbl
-  type free = (lexp, loc * lbl * t LEnv.t) result
-
-  type ctx = Free of (free -> continue) | Value of (lexp -> state)
-  and continue = t * ctx
-  and state = Halt of lexp | Continue of continue
-
-  let[@tail_mod_cons] rec reduce (A (env, exp), ctx) =
-    match Hashtbl.find label_table exp with
-    | LVar x -> (
-        match LEnv.find x env with
-        | exception Not_found -> (
-            match ctx with
-            | Free ctx -> reduce (ctx (Ok (Var (get_string x))))
-            | Value ctx -> (
-                match ctx (Var (get_string x)) with
-                | Halt e -> e
-                | Continue k -> reduce k))
-        | found -> reduce (found, ctx))
-    | LLam (x, e) -> (
-        match ctx with
-        | Free ctx -> reduce (ctx (Error (x, e, env)))
-        | Value ctx ->
-            let xs = get_string x in
-            reduce (A (LEnv.remove x env, e), Value (fun e -> ctx (Lam (xs, e))))
-        )
-    | LApp (e1, e2) ->
-        let ok_case =
-          match ctx with
-          | Free ctx -> fun e1 e2 -> Continue (ctx (Ok (App (e1, e2))))
-          | Value ctx -> fun e1 e2 -> ctx (App (e1, e2))
-        in
-        reduce
-          ( A (env, e1),
-            Free
-              (function
-              | Error (x, e, env1) -> (A (LEnv.add x (A (env, e2)) env1, e), ctx)
-              | Ok e1 -> (A (env, e2), Value (ok_case e1))) )
-
-  let rec pop_top_k l k =
-    match k with
-    | 0 -> l
-    | k when k > 0 -> (
-        match l with
-        | [] -> failwith "pop_top_k: empty list"
-        | _ :: tl -> pop_top_k tl (k - 1))
-    | _ -> failwith "pop_top_k: negative k"
-
-  type time = lbl * int
-
-  let init_time = (-1, 0)
-  let invalid_time = (-1, -1)
-
-  let print_time (t : time) =
-    let l, t = t in
-    print_string "(";
-    print_int l;
-    print_string ", ";
-    print_int t;
-    print_string ")"
-
-  let tick c _ t =
-    let _, t = t in
-    (c, t + 1)
-
-  let store : (time list, lbl * time list) Hashtbl.t = Hashtbl.create 10
-
-  let rec weak_reduce (c : lbl) (p : time list) (t : time) =
-    match Hashtbl.find label_table c with
-    | LVar _ ->
-        let addr = pop_top_k p (Hashtbl.find de_bruijn c) in
-        (Hashtbl.find store addr, t)
-    | LLam _ -> ((c, p), t)
-    | LApp (l1, l2) -> (
-        let (c1, p1), t1 = weak_reduce l1 p t in
-        let (c2, p2), t2 = weak_reduce l2 p t1 in
-        match Hashtbl.find label_table c1 with
-        | LLam (_, l) ->
-            let tick = tick c p t2 in
-            Hashtbl.replace store (tick :: p1) (c2, p2);
-            weak_reduce l (tick :: p1) tick
-        | _ -> failwith "free variables")
-
-  let rec recover_lexp (c : lbl) (p : time list) =
-    match Hashtbl.find label_table c with
-    | LVar x ->
-        let index = Hashtbl.find de_bruijn c in
-        let kth_time = List.nth p index in
-        if kth_time = invalid_time then Var (get_string x)
-        else
-          let c, p = Hashtbl.find store (pop_top_k p index) in
-          recover_lexp c p
-    | LLam (x, l) -> Lam (get_string x, recover_lexp l (invalid_time :: p))
-    | LApp (l1, l2) -> App (recover_lexp l1 p, recover_lexp l2 p)
-
-  let reduce_lexp e =
-    let my_lbl = label e LEnv.empty in
-    let () =
-      print_string
-        ("Number of syntactic locations: " ^ string_of_int !num_of_lbls ^ "\n")
-    in
-    let exp = reduce (A (LEnv.empty, my_lbl), Value (fun e -> Halt e)) in
-    let () =
-      print_string
-        ("Number of locations after evaluation: " ^ string_of_int !num_of_lbls
-       ^ "\n")
-    in
-    exp
-
-  let print_label_table () =
-    Hashtbl.iter
-      (fun l ->
-        print_int l;
-        print_string ": ";
-        function
-        | LVar x ->
-            print_string (get_string x);
-            print_newline ()
-        | LLam (x, e) ->
-            print_string ("\\" ^ get_string x ^ ".");
-            print_int e;
-            print_newline ()
-        | LApp (e1, e2) ->
-            print_int e1;
-            print_string "@";
-            print_int e2;
-            print_newline ())
-      label_table
-
-  let print_store t =
-    print_string "Number of applications: ";
-    print_time t;
-    print_newline ();
-    let join_table : (lbl list, (lbl * time list) list) Hashtbl.t =
-      Hashtbl.create 10
-    in
-    let update_join_table p_left (l, p_right) =
-      let lbl_list, _ = List.split p_left in
-      match Hashtbl.find join_table lbl_list with
-      | exception Not_found -> Hashtbl.add join_table lbl_list [ (l, p_right) ]
-      | original ->
-          Hashtbl.replace join_table lbl_list ((l, p_right) :: original)
-    in
-    let print_join_table list_left =
-      print_string "Joined from ";
-      List.iter
-        (fun l ->
-          print_int l;
-          print_string " ")
-        list_left;
-      print_newline ();
-      let print_entry list_right =
-        let print_list l =
-          List.iter
-            (fun t ->
-              print_time t;
-              print_string " ")
-            l
-        in
-        List.iter
-          (fun (l, p_right) ->
-            print_string "->";
-            print_int l;
-            print_string "/";
-            print_list p_right;
-            print_newline ())
-          list_right
-      in
-      print_entry
-    in
-    Hashtbl.iter update_join_table store;
-    Hashtbl.iter print_join_table join_table
-
-  let weak_reduce_lexp e =
-    let lbl = label e LEnv.empty in
-    let (c, p), t = weak_reduce lbl [] init_time in
-    print_store t;
-    recover_lexp c p
+module type Time = sig
+  type t
+  val tick : t ctx -> t -> string -> t expr_value -> t
+  val print : t -> unit
 end
 
-module Printer = struct
-  open Evaluator
+module Dom (T : sig 
+  type t 
+  val print : t -> unit
+end) = struct
+  module Mem = Map.Make(struct
+    type t = T.t
+    let compare = compare
+  end)
+  module ValSet = Set.Make(struct
+    type t = T.t expr_value
+    let compare = compare
+  end)
+  type context = T.t ctx (* type of my ctx *)
+  type memory = ValSet.t Mem.t (* type of my memory *)
+  type config = context * memory * T.t
+  type result = T.t value * memory * T.t
 
-  let rec finite_reduce leftover_steps (A (env, exp), ctx) =
-    if leftover_steps <= 0 then
-      let temp_var = Var ("[" ^ string_of_int exp ^ "]") in
-      match ctx with
-      | Value ctx -> (
-          match ctx temp_var with
-          | Halt e -> Pp.Pp.pp e
-          | Continue k -> finite_reduce leftover_steps k)
-      | Free ctx -> finite_reduce leftover_steps (ctx (Ok temp_var))
-    else
-      match Hashtbl.find label_table exp with
-      | LVar x -> (
-          match LEnv.find x env with
-          | exception Not_found -> (
-              match ctx with
-              | Free ctx ->
-                  finite_reduce (leftover_steps - 1)
-                    (ctx (Ok (Var (get_string x))))
-              | Value ctx -> (
-                  match ctx (Var (get_string x)) with
-                  | Halt e -> Pp.Pp.pp e
-                  | Continue k -> finite_reduce (leftover_steps - 1) k))
-          | found -> finite_reduce (leftover_steps - 1) (found, ctx))
-      | LLam (x, e) -> (
-          match ctx with
-          | Free ctx ->
-              finite_reduce (leftover_steps - 1) (ctx (Error (x, e, env)))
-          | Value ctx ->
-              let xs = get_string x in
-              finite_reduce (leftover_steps - 1)
-                (A (LEnv.remove x env, e), Value (fun e -> ctx (Lam (xs, e)))))
-      | LApp (e1, e2) ->
-          let ok_case =
-            match ctx with
-            | Free ctx -> fun e1 e2 -> Continue (ctx (Ok (App (e1, e2))))
-            | Value ctx -> fun e1 e2 -> ctx (App (e1, e2))
-          in
-          finite_reduce (leftover_steps - 1)
-            ( A (env, e1),
-              Free
-                (function
-                | Error (x, e, env1) ->
-                    ( A (LEnv.update x (fun _ -> Some (A (env, e2))) env1, e),
-                      ctx )
-                | Ok e1 -> (A (env, e2), Value (ok_case e1))) )
+  let rec print_ctx c =
+    match c with
+    | Hole -> print_string "[]"
+    | CLam (x, t, c) -> 
+      print_string "\\";
+      print_string x;
+      print_string ":";
+      T.print t;
+      print_string ".";
+      print_ctx c
+    | CLete (x, t, c) ->
+      print_string "let ";
+      print_string x;
+      print_string ":";
+      T.print t;
+      print_string " in ";
+      print_ctx c
+    | CLetm (m, cm, c) ->
+      print_string "let ";
+      print_string m;
+      print_string ":(";
+      print_ctx cm;
+      print_string ")";
+      print_string " in ";
+      print_ctx c
 
-  let finite_step steps pgm =
-    let () = print_endline "=========\nInput pgm\n=========" in
-    let () =
-      Pp.Pp.pp pgm;
-      print_newline ();
-      print_newline ()
-    in
-    let exp = label pgm LEnv.empty in
-    let () = print_endline "===========\nPartial pgm\n===========" in
-    finite_reduce steps (A (LEnv.empty, exp), Value (fun e -> Halt e));
-    print_newline ()
+  let print_expr_value v =
+    match v with
+    | Closure (x, e, c) ->
+      print_string "<\\";
+      print_string x;
+      print_string ".";
+      pp e;
+      print_string ", ";
+      print_ctx c;
+      print_string ">"
+
+  let print_value v =
+    match v with
+    | EVal v -> print_expr_value v
+    | MVal c -> print_ctx c
+
+  let print_valset (vs : ValSet.t) =
+    let vl = ValSet.elements vs in
+    print_string "{";
+    (match vl with
+    | [] -> ()
+    | v :: tl -> 
+      print_expr_value v;
+      List.iter (fun v -> print_string ", "; print_expr_value v) tl
+    ); print_string "}" 
+  
+  let print_mem (m : memory) =
+    let first = ref true in
+    Mem.iter (fun t vals ->
+      (if !first then first := false else print_string "U");
+      print_string "[";
+      T.print t;
+      print_string "|->";
+      print_valset vals;
+      print_string "]") m
+
+  let print_config (c, m, t) =
+    print_ctx c;
+    print_string ", ";
+    print_mem m;
+    print_string ", ";
+    T.print t
+  
+  let print_result (v, m, t) =
+    print_string "(";
+    print_value v;
+    print_string ", ";
+    print_mem m;
+    print_string ", ";
+    T.print t;
+    print_string ")"
+
+  let update_mem t vs (m : memory) =
+    Mem.update t 
+      (function
+      | None -> Some vs
+      | Some vals -> Some (ValSet.union vals vs)) m
+  
+  let compare_res r1 r2 =
+    match (r1, r2) with
+    | (v1, m1, t1), (v2, m2, t2) ->
+      let compv = compare v1 v2 in
+      let compm = Mem.compare ValSet.compare m1 m2 in
+      let compt = compare t1 t2 in
+      if compv < 0 then -1
+      else if compv > 0 then 1
+      else if compm < 0 then -1
+      else if compm > 0 then 1
+      else if compt < 0 then -1
+      else if compt > 0 then 1
+      else 0
+  
+  module ResSet = Set.Make(struct
+    type t = result
+    let compare = compare_res
+  end)
+  module Cache = Map.Make (struct
+    type t = tm * config
+    let compare (e1, s1) (e2, s2) =
+      let compe = compare e1 e2 in
+      let comps = compare_res s1 s2 in
+      if compe < 0 then -1
+      else if compe > 0 then 1
+      else if comps < 0 then -1
+      else if comps > 0 then 1
+      else 0
+  end)
+
+  let print_resset (vs : ResSet.t) =
+    let vl = ResSet.elements vs in
+    print_string "{";
+    (match vl with
+    | [] -> ()
+    | r :: tl -> 
+      print_result r;
+      List.iter (fun r -> print_string ", "; print_result r) tl
+    ); print_string "}" 
+
+  type cache = ResSet.t Cache.t
+  let update_cache (e, s) rs (a : cache) =
+    Cache.update (e, s) 
+      (function
+      | None -> Some rs
+      | Some res -> Some (ResSet.union res rs)) a
+  
+  let union_cache (a1 : cache) (a2 : cache) =
+    Cache.union (fun _ r1 r2 -> Some (ResSet.union r1 r2)) a1 a2
+
+  let print_cache (a : cache) =
+    Cache.iter (fun (e, cf) res ->
+      print_string "(";
+      pp e;
+      print_string ", ";
+      print_config cf;
+      print_string ")";
+      print_string "|->";
+      print_resset res;
+      print_newline ()) a
+end
+
+module Analyzer (T : Time) = struct
+  module Dom = Dom(T)
+  open Dom
+  let eval_cache (e : tm) (s : config) (a : cache) =
+    let delta = Cache.empty in
+    let (c, m, t) = s in
+    match e with
+    | EVar x -> (
+      match addr_x c x with
+      | None -> delta
+      | Some addr -> (
+        match Mem.find_opt addr m with
+        | None -> delta
+        | Some vals ->
+          let results = 
+            ResSet.of_list 
+            (List.map (fun v -> (EVal v, m, t)) (ValSet.elements vals))
+          in update_cache (e, s) results delta))
+    | Lam (x, e') -> 
+      let result = ResSet.singleton (EVal (Closure (x, e', c)), m, t) in
+      update_cache (e, s) result delta
+    | App (e1, e2) -> (
+      match Cache.find_opt (e1, s) a with
+      | None -> update_cache (e1, s) ResSet.empty delta
+      | Some res ->
+        ResSet.fold (fun res acc ->
+        match res with
+        | (EVal (Closure (x, e_lam, c_lam)), m', t') ->
+          (match Cache.find_opt (e2, (c, m', t')) a with
+          | None -> update_cache (e2, (c, m', t')) ResSet.empty acc
+          | Some res ->
+            ResSet.fold (fun res acc ->
+            match res with
+            | (EVal v, m'', t'') -> (
+              let t''' = T.tick c t'' x v in
+              let m''' = update_mem t'' (ValSet.singleton v) m'' in
+              let c''' = plugin c_lam (CLam (x, t'', Hole)) in
+              let s''' = (c''', m''', t''') in
+              match Cache.find_opt (e_lam, s''') a with
+              | None -> update_cache (e_lam, s''') ResSet.empty acc
+              | Some res -> update_cache (e, s) res acc)
+            | _ -> acc) res acc) 
+        | _ -> acc) res delta)
+    | Link (e1, e2) -> (
+      match Cache.find_opt (e1, s) a with
+      | None -> update_cache (e1, s) ResSet.empty delta
+      | Some res ->
+        ResSet.fold (fun res acc ->
+        match res with
+        | (MVal c', m', t') ->
+          let s' = (c', m', t') in
+          (match Cache.find_opt (e2, s') a with
+          | None -> update_cache (e2, s') ResSet.empty acc
+          | Some res -> update_cache (e, s) res acc)
+        | _ -> acc) res delta)
+    | Empty -> 
+      let result = ResSet.singleton (MVal c, m, t) in
+      update_cache (e, s) result delta
+    | MVar mv -> (
+      match ctx_M c mv with
+      | None -> delta
+      | Some cm -> 
+        let result = ResSet.singleton (MVal cm, m, t) in
+        update_cache (e, s) result delta)
+    | Lete (x, e1, e2) -> (
+      match Cache.find_opt (e1, s) a with
+      | None -> update_cache (e1, s) ResSet.empty delta
+      | Some res ->
+        ResSet.fold (fun res acc ->
+        match res with
+        | (EVal v, m', t') ->
+          let t'' = T.tick c t' x v in
+          let m'' = update_mem t' (ValSet.singleton v) m' in
+          let c'' = plugin c (CLete (x, t', Hole)) in
+          let s'' = (c'', m'', t'') in
+          (match Cache.find_opt (e2, s'') a with
+          | None -> update_cache (e2, s'') ResSet.empty acc
+          | Some res -> update_cache (e, s) res acc)
+        | _ -> acc) res delta)
+    | Letm (mv, e1, e2) -> (
+      match Cache.find_opt (e1, s) a with
+      | None -> update_cache (e1, s) ResSet.empty delta
+      | Some res ->
+        ResSet.fold (fun res acc ->
+        match res with
+        | (MVal cm, m', t') ->
+          let c' = plugin c (CLetm (mv, cm, Hole)) in
+          let s' = (c', m', t') in
+          (match Cache.find_opt (e2, s') a with
+          | None -> update_cache (e2, s') ResSet.empty acc
+          | Some res -> update_cache (e, s) res acc)
+        | _ -> acc) res delta)
+  
+  let rec fix (init : cache) =
+    let delta = 
+      Cache.fold 
+      (fun (e, s) _ acc -> union_cache acc (eval_cache e s init))
+      init Cache.empty in
+    let updated = union_cache init delta in
+    if (Cache.compare ResSet.compare init updated) = 0
+      then init
+      else fix updated
 end
