lib/lambda.ml
@@ -1,1 +1,90 @@
-type lexp = Var of string | Lam of string * lexp | App of lexp * lexp
+type tm = 
+  | EVar of string
+  | Lam of string * tm
+  | App of tm * tm
+  | Link of tm * tm
+  | Empty
+  | MVar of string
+  | Lete of string * tm * tm
+  | Letm of string * tm * tm
+
+type ('t1, 't2) link =
+  | BF of 't1
+  | AF of 't2
+
+type 't ctx =
+  | Hole
+  | CLam of string * 't * 't ctx
+  | CLete of string * 't * 't ctx
+  | CLetm of string * 't ctx * 't ctx
+
+type 't expr_value =
+  | Closure of string * tm * 't ctx
+
+type 't value =
+  | EVal of 't expr_value
+  | MVal of 't ctx
+
+let rec plugin (cout : 't ctx) (cin : 't ctx) =
+  match cout with
+  | Hole -> cin
+  | CLam (x, tx, c') -> CLam (x, tx, plugin c' cin)
+  | CLete (x, tx, c') -> CLete (x, tx, plugin c' cin)
+  | CLetm (m, cm, c') -> CLetm (m, cm, plugin c' cin)
+  
+let rec addr_x (c : 't ctx) (x : string) =
+  match c with
+  | Hole -> None
+  | CLam (x', tx', c')
+  | CLete (x', tx', c') ->
+    (match addr_x c' x with
+    | None -> if x = x' then (Some tx') else None
+    | addr -> addr)
+  | CLetm (_, _, c') -> addr_x c' x
+
+let rec ctx_M (c : 't ctx) (m : string) =
+  match c with
+  | Hole -> None
+  | CLam (_, _, c')
+  | CLete (_, _, c') -> ctx_M c' m
+  | CLetm (m', cm', c') -> (
+    match ctx_M c' m with
+    | None -> if m = m' then Some cm' else None
+    | cm -> cm)
+
+let rec map_inject (cout : 't ctx) (cin : 't ctx) =
+  match cin with
+  | Hole -> Hole
+  | CLam (x, t, c') -> CLam (x, t, map_inject cout c')
+  | CLete (x, t, c') -> CLete (x, t, map_inject cout c')
+  | CLetm (m, c', c'') -> CLetm (m, plugin cout (map_inject cout c'), map_inject cout c'')
+  
+let inject_ctx (cout : 't ctx) (cin : 't ctx) =
+  plugin cout (map_inject cout cin)
+
+let rec delete_prefix (cout : 't ctx) (cin : 't ctx) =
+  match cout, cin with
+  | Hole, cin -> cin
+  | CLam (x, t, cout'), CLam (x', t', cin')
+  | CLete (x, t, cout'), CLete(x', t', cin') ->
+    if x = x' && t = t' then
+      delete_prefix cout' cin'
+    else cin
+  | CLetm (m, cout', cout''), CLetm (m', cin', cin'') ->
+    if m = m' && cout' = cin' then
+      delete_prefix cout'' cin''
+    else cin
+  | _, _ -> cin
+
+let rec delete_map (cout : 't ctx) (cin : 't ctx) =
+  match cin with
+  | Hole -> Hole
+  | CLam (x, t, c') ->
+    CLam (x, t, delete_map cout c')
+  | CLete (x, t, c') ->
+    CLete (x, t, delete_map cout c')
+  | CLetm (m, c', c'') ->
+    CLetm (m, delete_map cout (delete_prefix cout c'), delete_map cout c'')
+
+let delete_ctx (cout : 't ctx) (cin : 't ctx) =
+  delete_map cout (delete_prefix cout cin)
