lib/parser.mly
@@ -8,7 +8,7 @@
 %right LP ID LAMBDA LET
 
 %start program
-%type <Lambda.lexp> program
+%type <Lambda.tm> program
 
 %%
 
@@ -16,13 +16,13 @@ program: exp EOF { $1 }
 
 exp :
 	| exp atom { Lambda.App ($1, $2) }
-        | atom { $1 }
+    | atom { $1 }
 	;
 
 atom :
-        | ID { Lambda.Var ($1) }
+    | ID { Lambda.EVar ($1) }
 	| LP exp RP { $2 }
 	| LAMBDA ID DOT exp %prec LP{ Lambda.Lam ($2, $4) }
 	| LET ID EQUAL exp IN exp %prec LP{ Lambda.App (Lambda.Lam ($2, $6), $4) }
-        ;
+    ;
 %%
