doc/coq/simple/Fixpoint.v
@@ -1,0 +1,106 @@
+From Simple Require Import Abstract.
+
+Generalizable Variables T.
+
+(* step_eval C st e v st' n : 
+    Given that \A{a} reached (C, st, e), the result (v, st') will be computed in n iterations *)
+Inductive step_eval `{time T} (C : @dy_ctx T) (st : @state T)
+    : tm -> dy_value -> state -> nat -> Prop :=
+  | s_var_e 
+    x v mem t addr
+    (STATE : ST mem t = st)
+    (ADDR : Some addr = addr_x C x)
+    (ACCESS : In v (mem addr))
+    : step_eval C st (e_var x) (EVal v) st 1
+  | s_lam x e
+    : step_eval C st (e_lam x e) (EVal (Closure x e C)) st 1
+  | s_app 
+    e1 e2 x e C_lam st_lam step1
+    arg mem t step2
+    v st_v step3
+    (FN : step_eval C st e1 (EVal (Closure x e C_lam)) st_lam step1)
+    (ARG : step_eval C st_lam e2 (EVal arg) (ST mem t) step2)
+    (BODY : step_eval (C_lam [|dy_c_lam x t ([||])|])
+                      (ST (t !#-> arg ; mem) (tick C (ST mem t) x arg))
+                      e (EVal v) st_v step3)
+    : step_eval C st (e_app e1 e2) (EVal v) st_v (4 + step1 + step2 + step3)
+  | s_link
+    m e C_m st_m step1 v st_v step2
+    (MOD : step_eval C st m (MVal C_m) st_m step1)
+    (LINK : step_eval C_m st_m e v st_v step2)
+    : step_eval C st (e_link m e) v st_v (3 + step1 + step2)
+  | s_empty
+    : step_eval C st m_empty (MVal C) st 1
+  | s_var_m
+    M C_M (ACCESS : Some C_M = ctx_M C M)
+    : step_eval C st (m_var M) (MVal C_M) st 1
+  | s_lete
+    x e v mem t step1
+    m C_m st_m step2
+    (EVALe : step_eval C st e (EVal v) (ST mem t) step1)
+    (EVALm : step_eval (C [|dy_c_lete x t ([||])|])
+                       (ST (t !#-> v ; mem) (tick C (ST mem t) x v))
+                       m (MVal C_m) st_m step2)
+    : step_eval C st (m_lete x e m) (MVal C_m) st_m (3 + step1 + step2)
+  | s_letm
+    M m' C' st' step1
+    m'' C'' st'' step2
+    (EVALm' : step_eval C st m' (MVal C') st' step1)
+    (EVALm'' : step_eval (C [|dy_c_letm M C' ([||])|]) st'
+                         m'' (MVal C'') st'' step2)
+    : step_eval C st (m_letm M m' m'') (MVal C'') st'' (3 + step1 + step2)
+.
+
+Inductive step_one `{time T} (C : @dy_ctx T) (st : @state T)
+    : tm -> dy_ctx -> state -> tm -> nat -> Prop :=
+  | s_appl 
+    e1 e2
+    : step_one C st (e_app e1 e2) C st e1 1
+  | s_appr
+    e1 e2 x e C_lam st_lam step1
+    (FN : step_eval C st e1 (EVal (Closure x e C_lam)) st_lam step1)
+    : step_one C st (e_app e1 e2) C st_lam e2 (2 + step1)
+  | s_appbody
+    e1 e2 x e C_lam st_lam step1
+    arg mem t step2
+    (FN : step_eval C st e1 (EVal (Closure x e C_lam)) st_lam step1)
+    (ARG : step_eval C st_lam e2 (EVal arg) (ST mem t) step2)
+    : step_one C st (e_app e1 e2) 
+               (C_lam [|dy_c_lam x t ([||])|])
+               (ST (t !#-> arg ; mem) (tick C (ST mem t) x arg))
+               e (3 + step1 + step2)
+  | s_linkl
+    m e
+    : step_one C st (e_link m e) C st m 1
+  | s_linkr
+    m e C_m st_m step1
+    (MOD : step_eval C st m (MVal C_m) st_m step1)
+    : step_one C st (e_link m e) C_m st_m e (2 + step1)
+  | s_letel
+    x e m
+    : step_one C st (m_lete x e m) C st e 1
+  | s_leter
+    x e m v mem t step1
+    (EVALe : step_eval C st e (EVal v) (ST mem t) step1)
+    : step_one C st (m_lete x e m)
+               (C [|dy_c_lete x t ([||])|])
+               (ST (t !#-> v ; mem) (tick C (ST mem t) x v))
+               m (2 + step1)
+  | s_letml
+    M m' m''
+    : step_one C st (m_letm M m' m'') C st m' 1
+  | s_letmr
+    M m' m'' C' st' step1
+    (EVALm' : step_eval C st m' (MVal C') st' step1)
+    : step_one C st (m_letm M m' m'') 
+               (C [|dy_c_letm M C' ([||])|]) st' m'' (2 + step1)
+.
+
+Inductive step_multi `{time T} (C : @dy_ctx T) (st : @state T)
+    : tm -> dy_ctx -> state -> tm -> nat -> Prop :=
+  | s_refl e : step_multi C st e C st e 0
+  | s_trans e C' st' e' step1 C'' st'' e'' step2
+            (STEP1 : step_one C st e C' st' e' step1)
+            (STEP2 : step_multi C' st' e' C'' st'' e'' step2)
+    : step_multi C st e C'' st'' e'' (step1 + step2)
+.
